src/impl/TLS13.Impl.Handle.ApplicationData.fsti
@@ -10,43 +10,73 @@ module C = TLS13.Impl.ConnectionState
 module CT = TLS13.Impl.Client.Types
 module L = TLS13.Impl.Messages
 module M = TLS13.Messages
+module Seq = FStar.Seq
 module SZ = FStar.SizeT
 module U8 = FStar.UInt8
+module WS = TLS13.Wire.Spec
 
 fn handle_application_data
   (c:C.connection_state)
-  (l:L.tls_message)
+  (content_type:U8.t)
+  (lapp:L.application_data)
   (raw:array U8.t)
   (raw_len:SZ.t)
+  (fragment:array U8.t)
+  (fragment_len:SZ.t)
   (network_out:array U8.t)
   (network_out_len:SZ.t)
   (app_out:array U8.t)
   (app_out_len:SZ.t)
   requires C.connection_exactly c 'st0 **
-           (exists* m. L.is_valid_tls_message l m) **
            pts_to raw 'raw_bytes **
+           pts_to fragment 'fragment_bytes **
+           (exists* m.
+            L.is_valid_tls_message (L.LTlsApplicationData lapp) m **
+            pure (CT.wire_parse_success content_type (Ghost.reveal 'fragment_bytes) m)) **
            pts_to network_out 'old_network_out **
            pts_to app_out 'old_app_out **
            pure (B.length 'raw_bytes == SZ.v raw_len /\
+                 B.length 'fragment_bytes == SZ.v fragment_len /\
                  B.length 'old_network_out == SZ.v network_out_len /\
-           B.length 'old_app_out == SZ.v app_out_len /\
-           L.tls_message_is_application_data l)
+                 B.length 'old_app_out == SZ.v app_out_len /\
+                 L.max_record_fragment_len <= SZ.v app_out_len /\
+                 CT.network_input_wf
+                   'st0
+                   content_type
+                   (Ghost.reveal 'fragment_bytes)
+                   (Ghost.reveal 'raw_bytes))
   returns resp: CT.client_response
-  ensures C.connection_exactly c (C.local_fail_state 'st0 C.tls_unexpected_message_error) **
+  ensures exists* st1 app_out_bytes.
+          C.connection_exactly c st1 **
           pts_to raw 'raw_bytes **
+          pts_to fragment 'fragment_bytes **
           pts_to network_out 'old_network_out **
-          pts_to app_out 'old_app_out **
+          pts_to app_out app_out_bytes **
           pure (B.length 'old_network_out == SZ.v network_out_len /\
-                B.length 'old_app_out == SZ.v app_out_len /\
-                CT.unexpected_message_response
-                  'st0
-                  (C.local_fail_state 'st0 C.tls_unexpected_message_error)
-                  resp
-                  'old_network_out
-                  'old_app_out /\
-                CT.some_legal_response
-                  'st0
-                  (C.local_fail_state 'st0 C.tls_unexpected_message_error)
-                  resp
-                  'old_network_out
-                  'old_app_out)
+               B.length app_out_bytes == SZ.v app_out_len /\
+               CT.legal_network_response
+                 'st0
+                 st1
+                 resp
+                 content_type
+                 (Ghost.reveal 'fragment_bytes)
+                 (Ghost.reveal 'raw_bytes)
+                 'old_network_out
+                 app_out_bytes /\
+               CT.some_legal_response
+                 'st0
+                 st1
+                 resp
+                 'old_network_out
+                 app_out_bytes /\
+               (resp.CT.status == CT.StepOk ==>
+                 exists bytes.
+                   CT.legal_received_tls_response
+                     'st0
+                     st1
+                     resp
+                     (M.TlsApplicationData bytes)
+                     (Ghost.reveal 'raw_bytes)
+                     'old_network_out
+                     app_out_bytes /\
+                   Seq.equal bytes (CT.response_app_out resp app_out_bytes)))
