src/impl/TLS13.Impl.Handle.Dispatch.fsti
@@ -60,6 +60,7 @@ fn dispatch_network_event
                  B.length 'fragment_bytes == SZ.v fragment_len /\
                  B.length 'old_network_out == SZ.v network_out_len /\
                  B.length 'old_app_out == SZ.v app_out_len /\
+                 L.max_record_fragment_len <= SZ.v app_out_len /\
                  CT.network_input_wf
                    'st0
                    content_type
